\documentclass{article} % For LaTeX2e
\usepackage{nips14submit_e,times}
\usepackage{amsmath}
\usepackage{amsthm}
\usepackage{amssymb}
\usepackage{mathtools}
\usepackage{hyperref}
\usepackage{url}
\usepackage{algorithm}
\usepackage[noend]{algpseudocode}
%\documentstyle[nips14submit_09,times,art10]{article} % For LaTeX 2.09

\usepackage{graphicx}
\usepackage{caption}
\usepackage{subcaption}

\def\eQb#1\eQe{\begin{eqnarray*}#1\end{eqnarray*}}
\def\eQnb#1\eQne{\begin{eqnarray}#1\end{eqnarray}}
\providecommand{\e}[1]{\ensuremath{\times 10^{#1}}}
\providecommand{\pb}[0]{\pagebreak}
\DeclarePairedDelimiter\ceil{\lceil}{\rceil}
\DeclarePairedDelimiter\floor{\lfloor}{\rfloor}

\newcommand{\E}{\mathrm{E}}
\newcommand{\Var}{\mathrm{Var}}
\newcommand{\Cov}{\mathrm{Cov}}

\def\Qb#1\Qe{\begin{question}#1\end{question}}
\def\Sb#1\Se{\begin{solution}#1\end{solution}}

\newenvironment{claim}[1]{\par\noindent\underline{Claim:}\space#1}{}
\newtheoremstyle{quest}{\topsep}{\topsep}{}{}{\bfseries}{}{ }{\thmname{#1}\thmnote{ #3}.}
\theoremstyle{quest}
\newtheorem*{definition}{Definition}
\newtheorem*{theorem}{Theorem}
\newtheorem*{lemma}{Lemma}
\newtheorem*{question}{Question}
\newtheorem*{preposition}{Preposition}
\newtheorem*{exercise}{Exercise}
\newtheorem*{challengeproblem}{Challenge Problem}
\newtheorem*{solution}{Solution}
\newtheorem*{remark}{Remark}
\usepackage{verbatimbox}
\usepackage{listings}
\usepackage{mathrsfs}
\title{Functional Analysis: \\
Problem Set I}


\author{
Youngduck Choi \\
CIMS \\
New York University\\
\texttt{yc1104@nyu.edu} \\
}


% The \author macro works with any number of authors. There are two commands
% used to separate the names and addresses of multiple authors: \And and \AND.
%
% Using \And between authors leaves it to \LaTeX{} to determine where to break
% the lines. Using \AND forces a linebreak at that point. So, if \LaTeX{}
% puts 3 of 4 authors names on the first line, and the last on the second
% line, try using \AND instead of \And before the third author name.

\newcommand{\fix}{\marginpar{FIX}}
\newcommand{\new}{\marginpar{NEW}}

\nipsfinalcopy % Uncomment for camera-ready version

\begin{document}


\maketitle

\begin{abstract}
This work contains solutions to the exercises of the problem set I.
\end{abstract}

\bigskip

\begin{question}[1]
\hfill
\begin{figure}[h!]
  \centering
    \includegraphics[width=0.7\textwidth]{funcA-h-e1-p1.png}
\end{figure}
\end{question}
\begin{solution} \hfill \\
First, define a map $\Phi:Y^{\perp} \to (E \setminus Y)^*$ naturally by
\eQb
f &\mapsto& ([x] \mapsto f(x))
\eQe 
where $[x] \in E\setminus Y$. The map is well-defined, because for any $[x] = [x']$,
\eQb
x' = x + y \>\> \text{for some} \>\> y \in Y \> \text{and} \>
f(x') = f(x) + f(y) = f(x).
\eQe
We now claim that $\Phi$ is a surjective isometry. By definition, for any $f \in
Y^{\perp}$,
\eQb
||\Phi(f)|| &=& \sup_{||[x]|| = 1} |<\Phi(f),[x]>| = \sup_{||[x]|| = 1} |<f,x>| \\
&=& \sup_{\inf_{y \in Y} ||x - y|| = 1} |<f,x>| 
\eQe 

\bigskip

For sake of completeness, we note that if both pre-image and image are Banach,
then a surjective isometry is a isometric isomorphism. This is a direct consequence
of open mapping theorem. First, isometry implies injectivity: for $T \in
\mathscr{L}(E,F)$ and $x,y \in E$, if $T(x) = T(y)$,
then $0 = ||T(x-y)|| = ||x-y||$, so $x = y$. Therefore, $T^{-1}$ is well-defined
as a map. Now, by open mapping theorem, we see that for any $O$ open in $E$,
$(T^{-1})^{-1}(O) = T(O)$ is open in $F$. Therefore, $T^{-1}$ is continuous as required.

\bigskip

It remains to be shown that $Y^{\perp}$ and $E \setminus Y$ are Banach. Suppose
$f \in E^*$ such that there exists $\{f_n\} \subset Y^{\perp}$ with $f_n \to f$. It
suffices to show that for any $y in Y$, we have $<f,y> = 0$. But this is true,
because norm convergence implies pointwise convergence and for all $n \geq 1$,
$<f_n,x> = 0$. Now, $E \setminus Y$ is Banach with respect to the quotient norm,
because  

\end{solution}

\newpage

\begin{question}[2]
\hfill
\begin{figure}[h!]
  \centering
    \includegraphics[width=0.7\textwidth]{funcA-h-e1-p2.png}
\end{figure}
\end{question}
\begin{solution} \hfill \\
\end{solution}

\newpage

\begin{question}[3]
\hfill
\begin{figure}[h!]
  \centering
    \includegraphics[width=0.7\textwidth]{funcA-h-e1-p3.png}
\end{figure}
\end{question}
\begin{solution} \hfill \\
\textbf{(i)} We prove the following generalization, known as the Riesz Lemma:
for each $\epsilon > 0$, there exists $x \in E$ such that $||x - y|| 
\geq 1 - \epsilon$, for any $y \in Y$. 

\smallskip

Let $0 < \epsilon < 1$. Let $x \in E\setminus Y$. As $Y$ is closed,
\eQb
d &:=& \text{dist}(x,Y) > 0.
\eQe
Choose $y^*$ in $Y$ such that 
\eQb
d \leq || x - y^* || \leq \dfrac{d}{1-\epsilon}. \>\>\> (1)
\eQe
Set $x^* = \dfrac{x-y^*}{||x-y^*||}$. Clearly, $||x^*|| = 1$, and,
for any $y \in Y$,
\eQb
||x^* - y|| &=& ||\dfrac{x-y^*}{||x-y^*||} - y|| = 
\dfrac{1}{||x-y^*||}||x- (y^* + y||x-y||^*)|| \\
&\geq&  \dfrac{d}{||x-y^*||} = 1-\epsilon, 
\eQe 
where the last inequality follows from $(1)$, and we are done.  

\bigskip

\textbf{(ii)} We proceed to construct a sequence $\{x_n\} \subset B_1$ 
such that there is no convergent subsequence, which shows that $B_1$ is not
compact in strong topology through sequential characterization of compactness
(strong topology is trivially metrizable). 

\smallskip
Choose any $x \in E$ such that $||x|| = 1$ and set $x_1 = x$. 
Then, for any $n$, using $(i)$, 
choose $x_n$ such that 
\eQb
||x_n|| = 1 \>\> \text{and}  \>\> ||x_n - y|| > \dfrac{1}{2}, 
\eQe
for any $y \in \text{span}(x_1,...,x_{n-1})$, where the validity comes from
the fact that any finite dimensional subspace is a proper, closed subspace
of an infinite dimensional space. Then, it is clear that $\{x_n\}$ has no
convergent subsequence, because for any $n \geq 1$, there exists $k, l \geq n$
with $k \neq l$, such that $||x_k - x_l|| > \dfrac{1}{2}$. Since being cauchy
is a necessary condition for being convergent, we are done. 
\hfill $\qed$ 

\end{solution}

\newpage

\begin{question}[4]
\hfill
\begin{figure}[h!]
  \centering
    \includegraphics[width=0.7\textwidth]{funcA-h-e1-p4.png}
\end{figure}
\end{question}
\begin{solution} \hfill \\
\textbf{(i)} 
Let $g$ be a bounded real-valued function and $\lambda > 0$. Then, by
linearity of Lebesgue integration,
\eQb
p(\lambda g) &=& \inf\{ l(h): \lambda g \leq h \in L^{\infty} \} \\
\lambda p(g) &=& \inf\{ l(\lambda h): g \leq h \in L^{\infty} \}.
\eQe
We claim that
\eQb
A := \{ l(h) : \lambda g \leq h \in L^{\infty} \} &=& 
\{ l(\lambda h): g \leq h \in L^{\infty} \} =: B
\eQe
If $\lambda g \leq h \in L^{\infty}$, 
then $ g \leq \dfrac{h}{\lambda} \in L^{\infty}$,
so $l(\lambda \dfrac{h}{\lambda}) = l(\lambda) \in B$. Conversely, if 
$ g \leq h \in L^{\infty}$ then, $\lambda g \leq \lambda h \in L^{\infty}$, 
so $l(\lambda h) \in A$. Hence, $p(\lambda g) = \lambda p(g)$. 

\smallskip

We now show that $p$ is sub-additive. Let $f,g$ be bounded real functions.
Then, for any $h_1, h_2 \in L^{\infty}$ such that $f \leq h_1$ and $g \leq h_2$,
\eQb
f+g &\leq& h_1 + h_2 \in L^{\infty},
\eQe
so, again by linearity of integration, 
\eQb
p(f+g) &\leq& l(h_1 + h_2) = l(h_1) + l(h_2). 
\eQe
Taking infs for $h_1$, then $h_2$, gives
\eQb
p(f+g) &\leq& p(f) + p(g), 
\eQe
as required.

\smallskip
 
For any $f,g$ bounded real-valued functions, 
\eQb
p(f+g) &=& \inf\{ l(f+g) : f+g \leq h , h \in L^{\infty}[0,1]\} \\ 
&=& \inf\{ l(f) + l(g) : f+g \leq h , h \in L^{\infty}[0,1]\}. 
\eQe
Suppose $g \leq 0$. Then, as $0 \in L^{\infty}[0,1]$ and $l(0) = 0$, by definition,
$p(g) \leq 0$. 

\smallskip

We show that $p(f) = l(f)$ if $f \in L^{\infty}[0,1]$. 
For all $h \in L^{\infty}[0,1]$ such that $f \leq h$, then, by monotonicity
of Lebesgue integration, $l(f) \leq l(h)$. Since $f \leq f$ trivially, it follows
that $p(f) = l(f)$. \hfill $\qed$

\bigskip

\textbf{(ii)}
Now, as $l = p$ on $L^{\infty}[0,1]$, by Hahn-Banach, $l$ can be extended to
the entire space of bounded real-valued functions. This shows that 
we can make sense of integration for any bounded functions in a weaker sense,
sacrificing some nice properties, such as countable additivity and so on(probably
if such properties hold, then it will contradict existence of non-measurable sets
by considering appropriate indicators). 
\hfill $\qed$ 
\end{solution}

\newpage

\begin{question}[5]
\hfill
\begin{figure}[h!]
  \centering
    \includegraphics[width=0.7\textwidth]{funcA-h-e1-p5.png}
\end{figure}
\end{question}
\begin{solution} \hfill \\
\end{solution}

\newpage

\begin{question}[6]
\hfill
\begin{figure}[h!]
  \centering
    \includegraphics[width=0.7\textwidth]{funcA-h-e1-p6.png}
\end{figure}
\end{question}
\begin{solution} \hfill \\
By ordinary properties of Minkowski functionals, it suffices to show that
for any $x \in E$ and $\lambda \in \mathbb{R}$,
\eQb
p(\lambda x) = |\lambda| p(x) \>\> &\text{and}& \>\>
p(x) = 0 \implies x = 0.
\eQe
We first prove the absolute homogeneity of $p$.
Now, if $\lambda \geq 0$,
then $p(\lambda x) = \lambda p(x)$ by positive homogeneity of Minkowski functionals.
Now, if $\lambda \geq 0$, then, by symmetry, and positive homogeneity again,
we obtain
\eQb
p(\lambda x) = p(-\lambda x) = -\lambda p(x), 
\eQe
which completes the proof of absolute homogeneity. 

\bigskip

Now, observe that, for any $0 <\alpha < \beta$, and $x \in E$, 
\eQb
\alpha^{-1}x \in C &\implies \beta^{-1}x \in C,
\eQe
because by convexity
\eQb
(1- \dfrac{\beta^{-1}}{\alpha^{-1}})0 + \dfrac{\beta^{-1}}{\alpha^{-1}}\alpha^{-1}x
= \beta^{-1}x \in C.
\eQe
Let $x \in E$ such that $p(x) = 0$, Then, by the above discussion,
it follows that
\eQb
\alpha^{-1}x &\in& C \>\>\> (*),
\eQe
for any $\alpha \in (0,\infty)$. Suppose $x \neq 0$, and let $r > 0$ 
large enough that $C \subset B(0,r)$. Then, it follows that, from $(*)$,
$\dfrac{r}{||x||}x \in C$, which contradicts the fact that $C \subset B(0,r)$.
Therefore, $x = 0$ and we are done. \hfill $\qed$
\end{solution}

\newpage

\begin{question}[7]
\hfill
\begin{figure}[h!]
  \centering
    \includegraphics[width=0.7\textwidth]{funcA-h-e1-p7.png}
\end{figure}
\end{question}
\begin{solution} \hfill \\

It is a well-known fact that $L^{\infty}$ is not separable. The proof can be
found in the Brezis textbook chapter 4.  
\end{solution} 


\end{document}
